lib/Qualify.thy
@@ -13,9 +13,11 @@ keywords "qualify" :: thy_decl and "end_qualify" :: thy_decl
 begin
 ML \<open>
 
+type qualify_args = {name : string, deep : bool}
+
 structure Data = Theory_Data
   (
-    type T = (theory * string) option * 
+    type T = (theory * qualify_args) option * 
              ((string * 
               ((binding Symtab.table) * (* facts *)
                (binding Symtab.table) * (* consts *)
@@ -51,37 +53,55 @@ fun map_consts_of str f thy = map_tabs_of str (@{apply 3(2)} f) thy;
 
 fun map_types_of str f thy = map_tabs_of str (@{apply 3(3)} f) thy;
 
-fun make_bind nm = 
+fun make_bind space thy nm = 
   let
-    val base = Long_Name.explode nm |> tl |> rev |> tl |> rev;
-  in fold (Binding.qualify false) base (Binding.make (Long_Name.base_name nm, Position.none)) end;
+    val short_name = 
+      Name_Space.extern_shortest (Proof_Context.init_global thy) space nm 
+      |> Long_Name.explode |> rev |> tl |> rev;
+    val long_name = Long_Name.explode nm |> tl |> rev |> tl |> rev;
+    
+    fun do_make_bind (short_qual :: l) (_ :: l') b = Binding.qualify true short_qual (do_make_bind l l' b)
+      | do_make_bind [] (long_qual :: l) b = Binding.qualify false long_qual (do_make_bind [] l b)
+      | do_make_bind [] [] b = b
+      | do_make_bind _ _ _ = raise Fail "Mismatched long and short identifiers"
+
+    val b = do_make_bind short_name long_name (Binding.make (Long_Name.base_name nm, Position.none))
+  
+  in b end;
 
 fun get_new_facts old_thy facts = 
-  Facts.dest_static false [Global_Theory.facts_of old_thy] facts
-  |> map (fn (nm, _) => `make_bind nm);
+  let
+    val space = Facts.space_of facts;
+  in
+     Facts.dest_static false [Global_Theory.facts_of old_thy] facts
+     |> map (fn (nm, _) => `(make_bind space old_thy) nm)
+  end
 
 fun get_new_consts old_thy consts =
   let
     val new_consts = #constants (Consts.dest consts)
     |> map fst;
+
+    val space = #const_space (Consts.dest consts);
     
     val consts = 
       filter (fn nm => not (can (Consts.the_const (Sign.consts_of old_thy)) nm) andalso
                        can (Consts.the_const consts) nm) new_consts
-      |> map (fn nm => `make_bind nm);
+      |> map (fn nm => `(make_bind space old_thy) nm);
 
   in consts end;
 
 fun get_new_types old_thy types =
   let
     val new_types = #types (Type.rep_tsig types);
+    val space = Name_Space.space_of_table new_types;
 
     val old_types = #types (Type.rep_tsig (Sign.tsig_of old_thy));
    
     val types = (new_types
       |> Name_Space.fold_table (fn (nm, _) => 
            not (Name_Space.defined old_types nm) ? cons nm)) []
-      |> map (fn nm => `make_bind nm);
+      |> map (fn nm => `(make_bind space old_thy) nm);
   in types end;
 
 fun add_qualified qual nm =
@@ -95,40 +115,46 @@ fun make_bind_local nm =
     val base = Long_Name.explode nm |> tl |> tl |> rev |> tl |> rev;
   in fold (Binding.qualify true) base (Binding.make (Long_Name.base_name nm, Position.none)) end;
 
-fun set_global_qualify str thy = 
+fun set_global_qualify (args : qualify_args) thy =
   let
+    val str = #name args
     val _ = Locale.check thy (str, Position.none)
     val _ = case get_qualify thy of SOME _ => error "Already in a qualify block!" | NONE => ();
+
+    val thy' = Data.map (apfst (K (SOME (thy,args)))) thy;
+
+  in if #deep args then
+  let
 
     val facts = 
       Facts.fold_static (fn (nm, _) => add_qualified str nm) (Global_Theory.facts_of thy) []
       |> map (`make_bind_local)
 
     val consts = fold (fn (nm, _) => add_qualified str nm) (#constants (Consts.dest (Sign.consts_of thy))) []
-      |> map (`make_bind_local)
+      |> map (`make_bind_local)                                                
 
     val types = 
       Name_Space.fold_table (fn (nm, _) => add_qualified str nm) (#types (Type.rep_tsig (Sign.tsig_of thy))) []
       |> map (`make_bind_local)
 
-
-    val thy' = thy
+    val thy'' = thy'
      |> map_facts_of str (fold (fn (b, nm) => (Symtab.update (nm, b))) facts)
      |> map_consts_of str (fold (fn (b, nm) => (Symtab.update (nm, b))) consts)
      |> map_types_of str (fold (fn (b, nm) => (Symtab.update (nm, b))) types)
 
-    val thy'' = thy'
-    |> Data.map (apfst (K (SOME (thy,str))))
-    |> fold (fn (nm, b) => Global_Theory.alias_fact b nm) (Symtab.dest (get_facts_of thy' str))
-    |> fold (fn (nm, b) => Sign.const_alias b nm) (Symtab.dest (get_consts_of thy' str))
-    |> fold (fn (nm, b) => Sign.type_alias b nm) (Symtab.dest (get_types_of thy' str))
+    val thy''' = thy''
+    |> fold (fn (nm, b) => Global_Theory.alias_fact b nm) (Symtab.dest (get_facts_of thy'' str))
+    |> fold (fn (nm, b) => Sign.const_alias b nm) (Symtab.dest (get_consts_of thy'' str))
+    |> fold (fn (nm, b) => Sign.type_alias b nm) (Symtab.dest (get_types_of thy'' str))
 
-  in thy'' end
+  in thy''' end
+  else thy'
+  end
 
 val _ =
   Outer_Syntax.command @{command_keyword qualify} "begin global qualification"
-    (Parse.name >> 
-      (fn str => Toplevel.theory (set_global_qualify str)));
+    (Parse.name -- Args.mode "deep">> 
+      (fn (str, deep) => Toplevel.theory (set_global_qualify {name = str, deep = deep})));
 
 fun syntax_alias global_alias local_alias b name =
   Local_Theory.declaration {syntax = true, pervasive = true} (fn phi =>
@@ -143,10 +169,12 @@ val type_alias = syntax_alias Sign.type_alias Proof_Context.type_alias;
 
 fun end_global_qualify thy =
   let
-    val (old_thy, nm) = 
+    val (old_thy, args) = 
       case get_qualify thy of
         SOME x => x 
       | NONE => error "Not in a global qualify"
+
+    val nm = #name args
 
     val facts = get_new_facts old_thy (Global_Theory.facts_of thy);
 
@@ -158,20 +186,25 @@ fun end_global_qualify thy =
     val thy' = thy
      |> map_facts_of nm (fold (fn (b, nm) => (Symtab.update (nm, b))) facts)
      |> map_consts_of nm (fold (fn (b, nm) => (Symtab.update (nm, b))) consts)
-     |> map_types_of nm (fold (fn (b, nm) => (Symtab.update (nm, b))) types)
-     |> (fn thy => fold (Global_Theory.hide_fact false o fst) (Symtab.dest (get_facts_of thy nm)) thy)
-     |> (fn thy => fold (Sign.hide_const false o fst) (Symtab.dest (get_consts_of thy nm)) thy)
-     |> (fn thy => fold (Sign.hide_type false o fst) (Symtab.dest (get_types_of thy nm)) thy)
-     |> Data.map (apfst (K NONE))
+     |> map_types_of nm (fold (fn (b, nm) => (Symtab.update (nm, b))) types);
 
-    val lthy = Named_Target.begin (nm, Position.none) thy';
+    val facts' = (if #deep args then (map swap (Symtab.dest (get_facts_of thy' nm))) else facts);
+    val consts' = (if #deep args then (map swap (Symtab.dest (get_consts_of thy' nm))) else consts);
+    val types' = (if #deep args then (map swap (Symtab.dest (get_types_of thy' nm))) else types);
+
+    val thy'' = thy'      
+     |> (fn thy => fold (Global_Theory.hide_fact false o snd) facts' thy)
+     |> (fn thy => fold (Sign.hide_const false o snd) consts' thy)
+     |> (fn thy => fold (Sign.hide_type false o snd) types' thy);
+
+    val lthy = Named_Target.begin (nm, Position.none) thy'';
 
     val lthy' = lthy
-      |> fold (uncurry fact_alias o swap) (Symtab.dest (get_facts_of thy' nm))
-      |> fold (uncurry const_alias o swap) (Symtab.dest (get_consts_of thy' nm))
-      |> fold (uncurry type_alias o swap) (Symtab.dest (get_types_of thy' nm));
+      |> fold (uncurry fact_alias) facts'
+      |> fold (uncurry const_alias) consts'
+      |> fold (uncurry type_alias) types';
 
-  in Local_Theory.exit_global lthy' end
+  in Local_Theory.exit_global lthy' |> Data.map (apfst (K NONE)) end
 
 val _ =
   Outer_Syntax.command @{command_keyword end_qualify} "end global qualification"
