proof/invariant-abstract/BCorres_AI.thy
@@ -203,6 +203,7 @@ lemma throw_on_false_bcorres[wp]: "bcorres f f' \<Longrightarrow>  bcorres (thro
   done
 
 context Arch begin
+  thm refl
   crunch (bcorres)bcorres[wp]: arch_finalise_cap truncate_state (simp: swp_def)
   unqualify_facts arch_finalise_cap_bcorres[wp]
 end
