proof/invariant-abstract/InvariantsPre_AI.thy
@@ -1,0 +1,142 @@
+(*
+ * Copyright 2014, General Dynamics C4 Systems
+ *
+ * This software may be distributed and modified according to the terms of
+ * the GNU General Public License version 2. Note that NO WARRANTY is provided.
+ * See "LICENSE_GPLv2.txt" for details.
+ *
+ * @TAG(GD_GPL)
+ *)
+
+theory InvariantsPre_AI
+imports LevityCatch_AI
+begin
+
+context Arch begin
+
+unqualify_types
+  aa_type
+
+unqualify_consts
+  aa_type :: "arch_kernel_obj \<Rightarrow> aa_type"
+
+end
+
+section "Locale Setup"
+
+locale pspace_update_eq' =
+  fixes f :: "'z::state_ext state \<Rightarrow> 'c::state_ext state"
+  assumes pspace: "kheap (f s) = kheap s"
+
+locale Arch_pspace_update_eq = pspace_update_eq'
+sublocale Arch_pspace_update_eq \<subseteq> Arch .
+
+locale pspace_update_eq = pspace_update_eq'
+
+
+locale arch_update_eq' =
+  fixes f :: "'z::state_ext state \<Rightarrow> 'c::state_ext state"
+  assumes arch: "arch_state (f s) = arch_state s"
+
+locale Arch_arch_update_eq = arch_update_eq'
+sublocale Arch_arch_update_eq \<subseteq> Arch .
+
+locale arch_update_eq = arch_update_eq'
+
+locale arch_idle_update_eq_more =
+  fixes f :: "'z::state_ext state \<Rightarrow> 'c::state_ext state"
+  assumes idle: "idle_thread (f s) = idle_thread s"
+  assumes irq: "interrupt_irq_node (f s) = interrupt_irq_node s"
+
+locale Arch_arch_idle_update_eq = Arch_arch_update_eq + arch_idle_update_eq_more
+sublocale Arch_arch_idle_update_eq \<subseteq> Arch .
+
+locale arch_idle_update_eq = arch_update_eq + arch_idle_update_eq_more
+
+
+locale Arch_p_arch_update_eq = Arch_pspace_update_eq + Arch_arch_update_eq
+sublocale Arch_p_arch_update_eq \<subseteq> Arch .
+
+locale p_arch_update_eq = pspace_update_eq + arch_update_eq
+
+locale Arch_p_arch_idle_update_eq = Arch_p_arch_update_eq + Arch_arch_idle_update_eq
+locale p_arch_idle_update_eq = p_arch_update_eq + arch_idle_update_eq
+
+locale Arch_p_arch_idle_update_int_eq = Arch_p_arch_idle_update_eq + Arch_pspace_update_eq
+
+section "Base definitions for Invariants"
+
+definition
+  obj_at :: "(Structures_A.kernel_object \<Rightarrow> bool) \<Rightarrow> obj_ref \<Rightarrow> 'z::state_ext state \<Rightarrow> bool"
+where
+  "obj_at P ref s \<equiv> \<exists>ko. kheap s ref = Some ko \<and> P ko"
+
+abbreviation
+  "ko_at k \<equiv> obj_at (op = k)"
+
+abbreviation
+  aobj_at :: "(arch_kernel_obj \<Rightarrow> bool) \<Rightarrow> obj_ref \<Rightarrow> 'z::state_ext state \<Rightarrow> bool"
+where
+  "aobj_at P ref s \<equiv> obj_at (\<lambda>ob. case ob of ArchObj aob \<Rightarrow> P aob | _ \<Rightarrow> False) ref s"
+
+lemma aobj_at_def:
+  "aobj_at P ref = (\<lambda>s. \<exists>ako. kheap s ref = Some (ArchObj ako) \<and> P ako)"
+  apply (rule ext)
+  apply (clarsimp simp add: obj_at_def)
+  apply (rule iffI)
+   apply clarsimp
+   apply (case_tac ko; clarsimp)
+   apply clarsimp
+  done
+
+abbreviation
+  "ako_at k \<equiv> aobj_at (op = k)"
+
+abbreviation
+  "atyp_at T \<equiv> aobj_at (\<lambda>ob. aa_type ob = T)"
+
+lemma obj_atE:
+  "\<lbrakk> obj_at P p s; \<And>ko. \<lbrakk> kheap s p = Some ko; P ko \<rbrakk> \<Longrightarrow> R \<rbrakk> \<Longrightarrow> R"
+  by (auto simp: obj_at_def)
+
+lemma obj_at_weakenE:
+  "\<lbrakk> obj_at P r s; \<And>ko. P ko \<Longrightarrow> P' ko \<rbrakk> \<Longrightarrow> obj_at P' r s"
+  by (clarsimp simp: obj_at_def)
+
+lemma ko_at_weakenE:
+  "\<lbrakk> ko_at k ptr s; P k \<rbrakk> \<Longrightarrow> obj_at P ptr s"
+  by (erule obj_at_weakenE, simp)
+
+lemma aobj_atE:
+  "\<lbrakk> aobj_at P p s; \<And>ko. \<lbrakk> kheap s p = Some (ArchObj ko); P ko \<rbrakk> \<Longrightarrow> R \<rbrakk> \<Longrightarrow> R"
+  by (auto simp: aobj_at_def)
+
+lemma aobj_at_weakenE:
+  "\<lbrakk> aobj_at P r s; \<And>ko. P ko \<Longrightarrow> P' ko \<rbrakk> \<Longrightarrow> aobj_at P' r s"
+  by (clarsimp simp: aobj_at_def)
+
+lemma ako_at_weakenE:
+  "\<lbrakk> ako_at k ptr s; P k \<rbrakk> \<Longrightarrow> aobj_at P ptr s"
+  by (erule aobj_at_weakenE, simp)
+
+definition
+  pspace_aligned :: "'z::state_ext state \<Rightarrow> bool"
+where
+  "pspace_aligned s \<equiv>
+     \<forall>x \<in> dom (kheap s). is_aligned x (obj_bits (the (kheap s x)))"
+
+lemma pspace_alignedD [intro?]:
+  "\<lbrakk> kheap s p = Some ko; pspace_aligned s \<rbrakk> \<Longrightarrow> is_aligned p (obj_bits ko)"
+  unfolding pspace_aligned_def by (drule bspec, blast, simp)
+
+text "objects don't overlap"
+definition
+  pspace_distinct :: "'z::state_ext state \<Rightarrow> bool"
+where
+  "pspace_distinct \<equiv>
+   \<lambda>s. \<forall>x y ko ko'. kheap s x = Some ko \<and> kheap s y = Some ko' \<and> x \<noteq> y \<longrightarrow>
+         {x .. x + (2 ^ obj_bits ko - 1)} \<inter>
+         {y .. y + (2 ^ obj_bits ko' - 1)} = {}"
+
+
+end
