spec/abstract/Decode_A.thy
@@ -23,15 +23,15 @@ imports
 begin
 
 unqualify_consts (in Arch)
- "ArchDefaultExtraRegisters :: arch_copy_register_sets"
- "check_valid_ipc_buffer :: vspace_ref \<Rightarrow> cap \<Rightarrow> (unit,'z::state_ext) se_monad"
- "is_valid_vtable_root :: cap \<Rightarrow> bool"
- "arch_decode_irq_control_invocation 
-   :: data \<Rightarrow> data list \<Rightarrow> cslot_ptr \<Rightarrow> cap list \<Rightarrow> (arch_irq_control_invocation,'z::state_ext) se_monad"
- "arch_data_to_obj_type :: nat \<Rightarrow> aobject_type option"
- "arch_decode_invocation ::
-    data \<Rightarrow> data list \<Rightarrow> cap_ref \<Rightarrow> cslot_ptr \<Rightarrow> arch_cap \<Rightarrow> (cap \<times> cslot_ptr) list \<Rightarrow> 
-     (arch_invocation,'z::state_ext) se_monad"
+ ArchDefaultExtraRegisters :: "arch_copy_register_sets"
+ check_valid_ipc_buffer :: "vspace_ref \<Rightarrow> cap \<Rightarrow> (unit,'z::state_ext) se_monad"
+ is_valid_vtable_root :: "cap \<Rightarrow> bool"
+ arch_decode_irq_control_invocation 
+  :: "data \<Rightarrow> data list \<Rightarrow> cslot_ptr \<Rightarrow> cap list \<Rightarrow> (arch_irq_control_invocation,'z::state_ext) se_monad"
+ arch_data_to_obj_type :: "nat \<Rightarrow> aobject_type option"
+ arch_decode_invocation ::
+   "data \<Rightarrow> data list \<Rightarrow> cap_ref \<Rightarrow> cslot_ptr \<Rightarrow> arch_cap \<Rightarrow> (cap \<times> cslot_ptr) list \<Rightarrow> 
+    (arch_invocation,'z::state_ext) se_monad"
           
 
 text {*
