spec/abstract/Retype_A.thy
@@ -23,10 +23,10 @@ imports
 begin
 
 unqualify_consts (in Arch)
-  "arch_default_cap :: aobject_type \<Rightarrow> obj_ref \<Rightarrow> nat \<Rightarrow> arch_cap"
-  "default_arch_object :: aobject_type \<Rightarrow> nat \<Rightarrow> arch_kernel_obj"
-  "init_arch_objects :: apiobject_type \<Rightarrow> obj_ref \<Rightarrow> nat \<Rightarrow> nat \<Rightarrow> obj_ref list \<Rightarrow> (unit,'z::state_ext) s_monad"
-
+  arch_default_cap :: "aobject_type \<Rightarrow> obj_ref \<Rightarrow> nat \<Rightarrow> arch_cap"
+  default_arch_object :: "aobject_type \<Rightarrow> nat \<Rightarrow> arch_kernel_obj"
+  init_arch_objects :: "apiobject_type \<Rightarrow> obj_ref \<Rightarrow> nat \<Rightarrow> nat \<Rightarrow> obj_ref list \<Rightarrow> (unit,'z::state_ext) s_monad"
+                                
 
 section "Creating Caps"
 
