spec/abstract/Schedule_A.thy
@@ -19,8 +19,8 @@ imports "./$L4V_ARCH/Arch_A"
 begin
 
 unqualify_consts (in Arch)
-  "arch_switch_to_thread :: obj_ref \<Rightarrow> (unit,'z::state_ext) s_monad"
-  "arch_switch_to_idle_thread :: (unit,'z::state_ext) s_monad"
+  arch_switch_to_thread :: "obj_ref \<Rightarrow> (unit,'z::state_ext) s_monad"
+  arch_switch_to_idle_thread :: "(unit,'z::state_ext) s_monad"
 
 abbreviation
   "idle st \<equiv> st = Structures_A.IdleThreadState"
