spec/abstract/Structures_A.thy
@@ -31,13 +31,13 @@ unqualify_types (in Arch)
         
 
 unqualify_consts (in Arch)
-  "acap_rights :: arch_cap \<Rightarrow> vm_rights"
-  "acap_rights_update :: vm_rights \<Rightarrow> arch_cap \<Rightarrow> arch_cap"
-  "arch_kobj_size :: arch_kernel_obj \<Rightarrow> nat"
-  "arch_obj_size :: arch_cap \<Rightarrow> nat"
-  "aobj_ref :: arch_cap \<rightharpoonup> obj_ref"
-  "asid_high_bits :: nat"
-  "asid_low_bits :: nat"
+  acap_rights :: "arch_cap \<Rightarrow> vm_rights"
+  acap_rights_update :: "vm_rights \<Rightarrow> arch_cap \<Rightarrow> arch_cap"
+  arch_kobj_size :: "arch_kernel_obj \<Rightarrow> nat"
+  arch_obj_size :: "arch_cap \<Rightarrow> nat"
+  aobj_ref :: "arch_cap \<rightharpoonup> obj_ref"
+  asid_high_bits :: "nat"
+  asid_low_bits :: "nat"
 
 
 
