spec/abstract/TcbAcc_A.thy
@@ -19,7 +19,7 @@ imports CSpace_A
 begin
 
 unqualify_consts (in Arch)
-  "in_user_frame :: obj_ref \<Rightarrow> 'z::state_ext state \<Rightarrow> bool"
+  in_user_frame :: "obj_ref \<Rightarrow> 'z::state_ext state \<Rightarrow> bool"
 
 text {* Store or load a word at an offset from an IPC buffer. *}
 definition
