spec/design/ARM/ArchLabelFuns_H.thy
@@ -13,9 +13,7 @@ chapter "Architecture-specific Invocation Label Functions"
 theory ArchLabelFuns_H
 imports "../InvocationLabels_H"
 begin
-
 context ARM begin
-
 text {*
   Arch-specific functions on invocation labels
 *}
@@ -41,6 +39,7 @@ where
       | ArchInvocationLabel ARMPageUnify_Instruction \<Rightarrow>   True
       | _ \<Rightarrow>   False
       )"
-end
 
+
+end
 end
