spec/design/skel/ARM/ArchLabelFuns_H.thy
@@ -13,11 +13,12 @@ chapter "Architecture-specific Invocation Label Functions"
 theory ArchLabelFuns_H
 imports "../InvocationLabels_H"
 begin
-
+context ARM begin
 text {*
   Arch-specific functions on invocation labels
 *}
 
 #INCLUDE_HASKELL SEL4/API/Invocation/ARM.lhs ONLY isPDFlushLabel isPageFlushLabel
 
+end
 end
